WIP

Traces.v
@@ -57,8 +57,7 @@ Inductive eqtrF (sim : trace A B -> trace A B -> Prop) :
 | EqTrTconsF a b tr1 tr2 (REL : sim tr1 tr2) :
   eqtrF sim (TconsF a b tr1) (TconsF a b tr2).
 
-Definition eqtr_ sim :
-  trace A B -> trace A B -> Prop :=
+Definition eqtr_ sim : trace A B -> trace A B -> Prop :=
   fun tr1 tr2 => eqtrF sim (observe tr1) (observe tr2).
 
 Lemma eqtrF_mono sim sim' tr tr'
@@ -92,4 +91,101 @@ Inductive eqtr_trans_clo (r : trace A B -> trace A B -> Prop)
       (REL: r tr1' tr2')
   : eqtr_trans_clo r tr1 tr2.
 
+Definition eqtrC := eqtr_trans_clo.
+
 End Eqtr.
+
+Require Import Program.Tactics.
+
+Ltac unfold_eqtr :=
+  (try match goal with [|- eqtr_ _ _ _] => red end);
+  (repeat match goal with [H: eqtr_ _ _ _ |- _ ] => red in H end).
+
+Tactic Notation "hinduction" hyp(IND) "before" hyp(H)
+  := move IND before H; revert_until IND; induction IND.
+
+Ltac inv H := inversion H; clear H; subst.
+
+Section EqTrProps.
+
+Context {A B : Type}.
+
+Lemma eqtrC_mon r1 r2 t1 t2
+      (IN: eqtrC r1 t1 t2)
+      (LE: r1 <2= r2):
+  @eqtrC A B r2 t1 t2.
+Proof.
+  destruct IN. econstructor; eauto.
+Qed.
+
+Hint Resolve eqtrC_mon : paco.
+
+Lemma eqtrC_wcompat :
+  wcompatible2 (@eqtr_ A B) eqtrC.
+Proof.
+  econstructor; [ eauto with paco | ].
+  intros. destruct PR.
+  punfold EQVl. punfold EQVr. unfold_eqtr.
+  hinduction REL before r; intros; clear tr1' tr2'.
+  - remember (TnilF a) as x.
+    hinduction EQVl before r; intros; subst; try inv Heqx; eauto.
+    remember (TnilF a0) as y.
+    hinduction EQVr before r; intros; subst; try inv Heqy.
+    constructor.
+  - remember (TauF m1) as x.
+    hinduction EQVl before r; intros; subst; try inv Heqx; try inv CHECK; [ | eauto with itree ].
+    remember (TauF m3) as y.
+    hinduction EQVr before r; intros; subst; try inv Heqy; try inv CHECK; [ | eauto with itree ].
+    pclearbot. econstructor. gclo.
+    econstructor; eauto with paco.
+  - remember (VisF e k1) as x.
+    hinduction EQVl before r; intros; try discriminate Heqx; [ inv_Vis | eauto with itree ].
+    remember (VisF e k3) as y.
+    hinduction EQVr before r; intros; try discriminate Heqy; [ inv_Vis | eauto with itree ].
+    econstructor. intros. pclearbot.
+    eapply MON.
+    + apply CMP. econstructor...
+    + intros. apply gpaco2_clo, PR.
+  - remember (TauF t1) as x.
+    hinduction EQVl before r; intros; subst; try inv Heqx; try inv CHECK; [ | eauto with itree ].
+    pclearbot. punfold REL...
+  - remember (TauF t2) as y.
+    hinduction EQVr before r; intros; subst; try inv Heqy; try inv CHECK; [ | eauto with itree ].
+    pclearbot. punfold REL...
+Qed.
+
+Hint Resolve eqitC_wcompat : paco.
+
+Lemma eqit_idclo_compat b1 b2: compose (eqitC b1 b2) id <3= compose id (eqitC b1 b2).
+Proof.
+  intros. apply PR.
+Qed.
+Hint Resolve eqit_idclo_compat : paco.
+
+Lemma eqitC_dist b1 b2:
+  forall r1 r2, eqitC b1 b2 (r1 \2/ r2) <2= (eqitC b1 b2 r1 \2/ eqitC b1 b2 r2).
+Proof.
+  intros. destruct PR. destruct REL; eauto with itree.
+Qed.
+
+Hint Resolve eqitC_dist : paco.
+
+Lemma eqit_clo_trans b1 b2 vclo
+      (MON: monotone2 vclo)
+      (CMP: compose (eqitC b1 b2) vclo <3= compose vclo (eqitC b1 b2)):
+  eqit_trans_clo b1 b2 false false <3= gupaco2 (eqit_ RR b1 b2 vclo) (eqitC b1 b2).
+Proof.
+  intros. destruct PR. gclo. econstructor; eauto with paco.
+Qed.
+
+Lemma eqtr_refl : forall (tr : trace A B), eqtr tr tr.
+Proof.
+red; intros.
+ginit.
+red.
+pcofix CIH. gstep; intros.
+intros; red.
+destruct tr.
+
+Lemma bisim_sym : forall tr1 tr2, bisim tr1 tr2 -> bisim tr2 tr1.
+Proof.
